some more cleanup.

theories/RTac/Instantiate.v
@@ -1,5 +1,6 @@
 Require Import ExtLib.Data.Sum.
 Require Import ExtLib.Tactics.
+Require Import MirrorCore.InstantiateI.
 Require Import MirrorCore.RTac.Core.
 Require Import MirrorCore.RTac.Simplify.
 
@@ -11,27 +12,27 @@ Set Strict Implicit.
 Section parameterized.
   Context {typ : Type}.
   Context {expr : Type}.
-  Context {subst : Type}.
   Context {RType_typ : RType typ}.
+  Context {RTypeOk_typ : RTypeOk}.
   Context {Expr_expr : Expr RType_typ expr}.
+  Context {ExprOk_expr : ExprOk Expr_expr}.
   Context {Typ0_Prop : Typ0 _ Prop}.
-  Context {Subst_subst : Subst subst expr}.
-  Context {SubstOk_subst : @SubstOk _ _ _ _ Expr_expr Subst_subst}.
 
   Variable instantiate : (nat -> option expr) -> nat -> expr -> expr.
+  Variable exprD'_instantiate
+  : @exprD'_instantiate _ _ _ _ instantiate.
 
-  Section instantiate.
-    Definition INSTANTIATE
-    : rtac typ expr subst :=
-      @SIMPLIFY typ expr subst _
-                (fun subst Subst_subst _ctx sub =>
-                   instantiate (fun u => subst_lookup u sub) 0).
-  End instantiate.
+  Definition INSTANTIATE
+  : rtac typ expr :=
+    @SIMPLIFY typ expr
+              (fun subst Subst_subst _ctx sub =>
+                 instantiate (fun u => subst_lookup u sub) 0).
 
-  Theorem INSTANTIATE_sound
-  : forall tus tvs, rtac_sound tus tvs INSTANTIATE.
+  Theorem INSTANTIATE_sound : rtac_sound INSTANTIATE.
   Proof.
     intros. eapply SIMPLIFY_sound.
+    intros; forward.
+    (** TODO: This needs higher-order instantiation *)
   Admitted.
 
 End parameterized.
